Centralize all of the make_array_naive running time stuff.

logical/make_array_naive.v
@@ -1,4 +1,5 @@
-Require Import Braun.common.braun Braun.common.log Braun.logical.insert Braun.common.util Braun.logical.index Braun.logical.list_util Braun.logical.sequence Braun.common.le_util.
+Require Import Braun.common.braun Braun.common.log Braun.common.util Braun.common.le_util Braun.common.array.
+Require Import Braun.logical.insert Braun.logical.index Braun.logical.list_util Braun.logical.sequence.
 Require Import Arith Arith.Even Arith.Div2 List.
 Require Import Program.
 Require Import Omega.
@@ -70,41 +71,6 @@ Proof.
   intros. eauto.
 Qed.
 Hint Resolve MakeArrayNaiveR_correct.
-
-Fixpoint man_time n : nat :=
-  match n with
-    | 0 => 0
-    | S n' => man_time n' + (cl_log n)
-  end.
-
-Example man_time_ex :
-  map man_time (1 :: 2 :: 3 :: 4 ::  5 ::  6 ::  7 ::  8 ::  9 :: 10 :: nil)
-  = (1 :: 3 :: 5 :: 8 :: 11 :: 14 :: 17 :: 21 :: 25 :: 29 :: nil).
-Proof.
-  auto.
-Qed.
-
-Lemma man_time_nlogn :
-  forall n,
-    man_time n <= n * cl_log n.
-Proof.
-  induction n as [|n].
-
-  simpl; omega.
-
-  replace (S n * cl_log (S n)) with (n * cl_log (S n) + cl_log (S n));
-    [|unfold mult; fold mult; omega].
-  unfold man_time; fold man_time.
-  apply le_plus_left.
-  apply (le_trans (man_time n)
-                  (n * cl_log n)
-                  (n * cl_log (S n))).
-  assumption.
-  
-  apply le_mult_right.
-  apply cl_log_monotone.
-Qed.
-Hint Resolve man_time_nlogn.
 
 Theorem MakeArrayNaiveR_time :
   forall A xs (bt:@bin_tree A) t,
