omonad/make_array.v
@@ -1,5 +1,6 @@
 Require Import Braun.common.le_util Braun.common.log.
 Require Import Braun.omonad.braun Braun.omonad.monad Braun.omonad.insert.
+Require Import Braun.common.array.
 Require Import Program.Equality Omega.
 Require Import Div2 List.
 Set Implicit Arguments.
@@ -28,48 +29,16 @@ End ifoldr.
 
 Section make_array_naive.
   Variable A : Set.
-
-  (* Not sure how to prove this is O(nlogn) *)
-  Fixpoint rt_naive n : nat :=
-    match n with
-      | 0 => 0
-      | S n' => rt_naive n' + (cl_log n)
-    end.
-
-  Example rt_naive_ex :
-    map rt_naive (1 :: 2 :: 3 :: 4 ::  5 ::  6 ::  7 ::  8 ::  9 :: 10 :: nil)
-               = (1 :: 3 :: 5 :: 8 :: 11 :: 14 :: 17 :: 21 :: 25 :: 29 :: nil).
-  compute; reflexivity. Qed.
   
   Program Definition make_array_naive n (s : ilist A n)
-  : C (braun_tree A n) (rt_naive n) :=
-    ifoldr (fun n => C (braun_tree A n) (rt_naive n))
+  : C (braun_tree A n) (man_time n) :=
+    ifoldr (fun n => C (braun_tree A n) (man_time n))
            (fun n x ct => ct >>= insert x)
            (ret Empty)
            s.
   Obligation 1. omega. Qed.
   Obligation 2.
   replace (n0 + 1) with (S n0);[reflexivity|omega]. 
-  Qed.
-
-  Lemma rt_naive_is_nlogn : forall n, rt_naive n <= n * cl_log n.
-    apply (well_founded_ind 
-             lt_wf 
-             (fun n => rt_naive n <= n * cl_log n)).
-    intros x IND.
-    destruct x.
-    compute; constructor.
-    replace (rt_naive (S x)) with (rt_naive x + cl_log (S x));[|simpl;reflexivity].
-    replace (S x * cl_log (S x)) with (cl_log (S x) + x * cl_log (S x));[|simpl;omega].
-    rewrite plus_comm.
-    apply le_plus_right.
-    apply (le_trans (rt_naive x) 
-                    (x * cl_log x)
-                    (x * cl_log (S x))).
-    apply IND.
-    constructor.
-    apply le_mult_right.
-    apply cl_log_monotone.
   Qed.
 
 End make_array_naive.
